Foundation/IntProp/Kripke2/Hilbert/Cl.lean
@@ -3,7 +3,9 @@ import Foundation.IntProp.Kripke2.Hilbert.Soundness
 
 namespace LO.IntProp
 
+open Kripke
 open Formula.Kripke
+
 
 abbrev Kripke.EuclideanFrameClass : FrameClass := { F | Euclidean F }
 
@@ -31,7 +33,7 @@ instance : Kripke.EuclideanFrameClass.DefinedByFormula (Axioms.LEM (.atom 0)) :=
 ⟩
 
 instance : Kripke.EuclideanFrameClass.IsNonempty := ⟨by
-  use ⟨Unit, λ _ _ => True, by simp [Reflexive], by simp [Transitive]⟩;
+  use pointFrame;
   simp [Euclidean];
 ⟩
 
@@ -47,6 +49,57 @@ instance sound : Sound Hilbert.Cl EuclideanFrameClass := inferInstance
 instance consistent : System.Consistent Hilbert.Cl := Kripke.Hilbert.consistent_of_FrameClass EuclideanFrameClass
 
 end Hilbert.Cl.Kripke
+
+
+
+
+namespace Kripke
+
+abbrev ClassicalValuation := ℕ → Prop
+
+end Kripke
+
+
+namespace Formula.Kripke
+
+open IntProp.Kripke
+
+abbrev ClassicalSatisfies (V : ClassicalValuation) (φ : Formula ℕ) : Prop := Satisfies (⟨pointFrame, ⟨λ _ => V, by tauto⟩⟩) () φ
+
+namespace ClassicalSatisfies
+
+instance : Semantics (Formula ℕ) (ClassicalValuation) := ⟨ClassicalSatisfies⟩
+
+variable {V : ClassicalValuation} {a : ℕ}
+
+@[simp] lemma atom_def : V ⊧ atom a ↔ V a := by simp only [Semantics.Realize, Satisfies]
+
+instance : Semantics.Tarski (ClassicalValuation) where
+  realize_top := by simp [Semantics.Realize, ClassicalSatisfies, Satisfies];
+  realize_bot := by simp [Semantics.Realize, ClassicalSatisfies, Satisfies];
+  realize_or  := by simp [Semantics.Realize, ClassicalSatisfies, Satisfies];
+  realize_and := by simp [Semantics.Realize, ClassicalSatisfies, Satisfies];
+  realize_imp := by simp [Semantics.Realize, Satisfies]; tauto;
+  realize_not := by simp [Semantics.Realize, Satisfies]; tauto;
+
+end ClassicalSatisfies
+
+end Formula.Kripke
+
+
+namespace Hilbert.Cl
+
+lemma classical_sound : (Hilbert.Cl) ⊢! φ → (∀ V : ClassicalValuation, V ⊧ φ) := by
+  intro h V;
+  apply Hilbert.Cl.Kripke.sound.sound h Kripke.pointFrame;
+  simp [Euclidean];
+
+lemma unprovable_of_exists_classicalValuation : (∃ V : ClassicalValuation, ¬(V ⊧ φ)) → (Hilbert.Cl) ⊬ φ := by
+  contrapose;
+  simp;
+  apply classical_sound;
+
+end Hilbert.Cl
 
 
 end LO.IntProp
