Foundation/IntProp/ConsistentTableau.lean
@@ -1,0 +1,447 @@
+import Foundation.IntProp.Formula
+import Foundation.Logic.HilbertStyle.Supplemental
+
+namespace LO.IntProp
+
+open System FiniteContext
+open Formula
+
+variable {α : Type*}
+variable {S} [System (Formula α) S]
+variable {𝓢 : S}
+
+
+def Tableau (α : Type u) := Set (Formula α) × Set (Formula α)
+
+
+namespace Tableau
+
+variable {φ ψ: Formula α} {T U : FormulaSet α} {t u : Tableau α}
+
+abbrev Consistent (𝓢 : S) (t : Tableau α) := ∀ {Γ Δ : List (Formula α)}, (∀ φ ∈ Γ, φ ∈ t.1) → (∀ φ ∈ Δ, φ ∈ t.2) → 𝓢 ⊬ ⋀Γ ➝ ⋁Δ
+
+abbrev Inconsistent (𝓢 : S) (t : Tableau α) := ¬Consistent 𝓢 t
+
+instance : HasSubset (Tableau α) := ⟨λ t₁ t₂ => t₁.1 ⊆ t₂.1 ∧ t₁.2 ⊆ t₂.2⟩
+@[simp] lemma subset_def {t₁ t₂ : Tableau α} : t₁ ⊆ t₂ ↔ t₁.1 ⊆ t₂.1 ∧ t₁.2 ⊆ t₂.2 := by rfl
+
+@[simp] lemma equality_def {t₁ t₂ : Tableau α} : t₁ = t₂ ↔ t₁.1 = t₂.1 ∧ t₁.2 = t₂.2 := by
+  constructor;
+  . intro h; cases h; simp;
+  . rintro ⟨h₁, h₂⟩; cases t₁; cases t₂; simp_all;
+
+lemma not_mem₂ (hCon : t.Consistent 𝓢) {Γ : List (Formula α)} (hΓ : ∀ φ ∈ Γ, φ ∈ t.1) (h : 𝓢 ⊢! ⋀Γ ➝ ψ) : ψ ∉ t.2 := by
+  by_contra hC;
+  have : 𝓢 ⊢! ⋀Γ ➝ ⋁[ψ] := by simpa;
+  have : 𝓢 ⊬ ⋀Γ ➝ ⋁[ψ] := hCon (by aesop) (by aesop);
+  contradiction;
+
+section
+
+variable [System.Intuitionistic 𝓢]
+
+lemma disjoint_of_consistent (hCon : t.Consistent 𝓢) : Disjoint t.1 t.2 := by
+  by_contra h;
+  obtain ⟨T, hp₁, hp₂, hp⟩ := by simpa [Disjoint] using h;
+  obtain ⟨φ, hp⟩ := Set.nonempty_def.mp $ Set.nonempty_iff_ne_empty.mpr hp;
+  simp [Consistent] at hCon;
+  have : 𝓢 ⊬ ⋀[φ] ➝ ⋁[φ] := hCon
+    (by simp_all; apply hp₁; assumption)
+    (by simp_all; apply hp₂; assumption);
+  have : 𝓢 ⊢! ⋀[φ] ➝ ⋁[φ] := by simp;
+  contradiction;
+
+variable [DecidableEq α]
+
+lemma iff_consistent_insert₁
+  : Tableau.Consistent 𝓢 ((insert φ T), U) ↔ ∀ {Γ Δ : List (Formula α)}, (∀ φ ∈ Γ, φ ∈ T) → (∀ φ ∈ Δ, φ ∈ U) → 𝓢 ⊬ φ ⋏ ⋀Γ ➝ ⋁Δ := by
+  constructor;
+  . intro h Γ Δ hΓ hΔ;
+    by_contra hC;
+    have : 𝓢 ⊬ ⋀(φ :: Γ) ➝ ⋁Δ := h (by simp; intro ψ hq; right; exact hΓ ψ hq;) hΔ;
+    have : 𝓢 ⊢! ⋀(φ :: Γ) ➝ ⋁Δ := iff_imply_left_cons_conj'!.mpr hC;
+    contradiction;
+  . intro h Γ Δ hΓ hΔ;
+    simp_all only [Set.mem_insert_iff];
+    have : 𝓢 ⊬ φ ⋏ ⋀(Γ.remove φ) ➝ ⋁Δ := h (by
+      intro ψ hq;
+      have := by simpa using hΓ ψ $ List.mem_of_mem_remove hq;
+      cases this with
+      | inl h => simpa [h] using List.mem_remove_iff.mp hq;
+      | inr h => assumption;
+    ) hΔ;
+    by_contra hC;
+    have : 𝓢 ⊢! φ ⋏ ⋀(Γ.remove φ) ➝ ⋁Δ := imp_trans''! and_comm! $ imply_left_remove_conj! (φ := φ) hC;
+    contradiction;
+
+lemma iff_not_consistent_insert₁ : ¬Tableau.Consistent 𝓢 ((insert φ T), U) ↔ ∃ Γ Δ : List (Formula α), (∀ φ ∈ Γ, φ ∈ T) ∧ (∀ φ ∈ Δ, φ ∈ U) ∧ 𝓢 ⊢! φ ⋏ ⋀Γ ➝ ⋁Δ := by
+  constructor;
+  . contrapose; push_neg; apply iff_consistent_insert₁.mpr;
+  . contrapose; push_neg; apply iff_consistent_insert₁.mp;
+
+lemma iff_consistent_insert₂ : Tableau.Consistent 𝓢 (T, (insert φ U)) ↔ ∀ {Γ Δ : List (Formula α)}, (∀ φ ∈ Γ, φ ∈ T) → (∀ φ ∈ Δ, φ ∈ U) → 𝓢 ⊬ ⋀Γ ➝ φ ⋎ ⋁Δ := by
+  constructor;
+  . intro h Γ Δ hΓ hΔ;
+    by_contra hC;
+    have : 𝓢 ⊬ ⋀Γ ➝ ⋁(φ :: Δ) := h hΓ (by simp; intro ψ hq; right; exact hΔ ψ hq);
+    have : 𝓢 ⊢! ⋀Γ ➝ ⋁(φ :: Δ) := implyRight_cons_disj!.mpr hC;
+    contradiction;
+  . intro h Γ Δ hΓ hΔ;
+    simp_all;
+    have : 𝓢 ⊬ ⋀Γ ➝ φ ⋎ ⋁(Δ.remove φ) := h hΓ (by
+      intro ψ hq;
+      have := by simpa using hΔ ψ $ List.mem_of_mem_remove hq;
+      cases this with
+      | inl h => simpa [h] using List.mem_remove_iff.mp hq;
+      | inr h => assumption;
+    );
+    by_contra hC;
+    have : 𝓢 ⊢! ⋀Γ ➝ φ ⋎ ⋁(Δ.remove φ) := imp_trans''! hC $ forthback_disj_remove;
+    contradiction;
+
+lemma iff_not_consistent_insert₂ : ¬Tableau.Consistent 𝓢 (T, (insert φ U)) ↔ ∃ Γ Δ : List (Formula α), (∀ φ ∈ Γ, φ ∈ T) ∧ (∀ φ ∈ Δ, φ ∈ U) ∧ 𝓢 ⊢! ⋀Γ ➝ φ ⋎ ⋁Δ := by
+  constructor;
+  . contrapose; push_neg; apply iff_consistent_insert₂.mpr;
+  . contrapose; push_neg; apply iff_consistent_insert₂.mp;
+
+section Consistent
+
+variable {t : Tableau α}
+
+lemma consistent_either (hCon : t.Consistent 𝓢) (φ : Formula α) : Tableau.Consistent 𝓢 ((insert φ t.1), t.2) ∨ Tableau.Consistent 𝓢 (t.1, (insert φ t.2)) := by
+  by_contra hC;
+  push_neg at hC;
+  have ⟨hC₁, hC₂⟩ := hC;
+
+  obtain ⟨Γ₁, Δ₁, hΓ₁, hΔ₁, h₁⟩ := iff_not_consistent_insert₁.mp hC₁;
+  replace h₁ := imply_left_and_comm'! h₁;
+
+  obtain ⟨Γ₂, Δ₂, hΓ₂, hΔ₂, h₂⟩ := iff_not_consistent_insert₂.mp hC₂;
+
+  have : 𝓢 ⊢! ⋀(Γ₁ ++ Γ₂) ➝ ⋁(Δ₁ ++ Δ₂) := imp_trans''! (and₁'! iff_concat_conj!) $ imp_trans''! (cut! h₁ h₂) (and₂'! iff_concact_disj!);
+  have : 𝓢 ⊬ ⋀(Γ₁ ++ Γ₂) ➝ ⋁(Δ₁ ++ Δ₂) := hCon (by simp; rintro ψ (hq₁ | hq₂); exact hΓ₁ ψ hq₁; exact hΓ₂ ψ hq₂) (by simp; rintro ψ (hq₁ | hq₂); exact hΔ₁ ψ hq₁; exact hΔ₂ ψ hq₂);
+  contradiction;
+
+end Consistent
+
+end
+
+
+abbrev Saturated (t : Tableau α) := ∀ φ : Formula α, φ ∈ t.1 ∨ φ ∈ t.2
+
+section Saturated
+
+variable [System.Intuitionistic 𝓢]
+variable {t : Tableau α}
+
+lemma mem₂_of_not_mem₁ (hMat : Saturated t) : φ ∉ t.1 → φ ∈ t.2 := by
+  intro h;
+  cases (hMat φ) with
+  | inl h' => exact absurd h' h;
+  | inr _ => assumption;
+
+lemma mem₁_of_not_mem₂ (hMat : Saturated t) : φ ∉ t.2 → φ ∈ t.1 := by
+  intro h;
+  cases (hMat φ) with
+  | inl _ => assumption;
+  | inr h' => exact absurd h' h;
+
+
+lemma not_mem₁_iff_mem₂ (hCon : t.Consistent 𝓢) (hMat : Saturated t) : φ ∉ t.1 ↔ φ ∈ t.2 := by
+  constructor;
+  . apply mem₂_of_not_mem₁ hMat;
+  . apply Set.disjoint_right.mp $ disjoint_of_consistent hCon;
+
+lemma not_mem₂_iff_mem₁ (hCon : t.Consistent 𝓢) (hMat : Saturated t) : φ ∉ t.2 ↔ φ ∈ t.1 := by
+  constructor;
+  . apply mem₁_of_not_mem₂ hMat;
+  . apply Set.disjoint_left.mp $ disjoint_of_consistent hCon;
+
+lemma saturated_duality
+  {t₁ t₂ : Tableau α}
+  (ct₁ : t₁.Consistent 𝓢) (ct₂ : t₂.Consistent 𝓢)
+  (st₁ : Saturated t₁) (st₂ : Saturated t₂)
+  : t₁.1 = t₂.1 ↔ t₁.2 = t₂.2 := by
+  constructor;
+  . intro h;
+    apply Set.eq_of_subset_of_subset;
+    . intro φ hp;
+      apply not_mem₁_iff_mem₂ ct₂ st₂ |>.mp; rw [←h];
+      apply not_mem₁_iff_mem₂ ct₁ st₁ |>.mpr hp;
+    . intro φ hp;
+      apply not_mem₁_iff_mem₂ ct₁ st₁ |>.mp; rw [h];
+      apply not_mem₁_iff_mem₂ ct₂ st₂ |>.mpr hp;
+  . intro h;
+    apply Set.eq_of_subset_of_subset;
+    . intro φ hp;
+      apply not_mem₂_iff_mem₁ ct₂ st₂ |>.mp; rw [←h];
+      apply not_mem₂_iff_mem₁ ct₁ st₁ |>.mpr hp;
+    . intro φ hp;
+      apply not_mem₂_iff_mem₁ ct₁ st₁ |>.mp; rw [h];
+      apply not_mem₂_iff_mem₁ ct₂ st₂ |>.mpr hp;
+
+end Saturated
+
+lemma emptyset_consistent [System.Intuitionistic 𝓢] [DecidableEq α] [H_consis : System.Consistent 𝓢] : Consistent 𝓢 ⟨∅, ∅⟩ := by
+  intro Γ Δ hΓ hΔ;
+  replace hΓ : Γ = [] := List.eq_nil_iff_forall_not_mem.mpr hΓ;
+  replace hΔ : Δ = [] := List.eq_nil_iff_forall_not_mem.mpr hΔ;
+  subst hΓ hΔ;
+  by_contra hC;
+  simp at hC;
+  obtain ⟨ψ, hq⟩ := H_consis.exists_unprovable;
+  have : 𝓢 ⊢! ψ := efq'! (hC ⨀ imp_id!);
+  contradiction;
+
+section lindenbaum
+
+variable (𝓢 : S)
+variable {t : Tableau α}
+
+open Classical
+open Encodable
+
+def lindenbaum_next (φ : Formula α) (t : Tableau α) : Tableau α := if Tableau.Consistent 𝓢 (insert φ t.1, t.2) then (insert φ t.1, t.2) else (t.1, insert φ t.2)
+
+def lindenbaum_next_indexed [Encodable α] (t : Tableau α) : ℕ → Tableau α
+  | 0 => t
+  | i + 1 =>
+    match (decode i) with
+    | some φ => (lindenbaum_next_indexed t i).lindenbaum_next 𝓢 φ
+    | none => lindenbaum_next_indexed t i
+local notation:max t"[" i "]" => lindenbaum_next_indexed 𝓢 t i
+
+def lindenbaum_maximal [Encodable α] (t : Tableau α) : Tableau α := (⋃ i, t[i].1, ⋃ i, t[i].2)
+local notation:max t"∞" => lindenbaum_maximal 𝓢 t
+
+@[simp] lemma lindenbaum_next_indexed_zero [Encodable α] {t : Tableau α} : (t.lindenbaum_next_indexed 𝓢 0) = t := by simp [lindenbaum_next_indexed]
+
+
+variable {𝓢}
+
+lemma next_parametericConsistent [System.Intuitionistic 𝓢] (consistent : t.Consistent 𝓢) (φ : Formula α) : (t.lindenbaum_next 𝓢 φ).Consistent 𝓢 := by
+  simp [lindenbaum_next];
+  split;
+  . simpa;
+  . rcases (consistent_either consistent φ) with (h | h);
+    . contradiction;
+    . assumption;
+
+variable [Encodable α]
+
+lemma lindenbaum_next_indexed_parametricConsistent_succ [System.Intuitionistic 𝓢] {i : ℕ} : Consistent 𝓢 t[i] → Consistent 𝓢 t[i + 1] := by
+  simp [lindenbaum_next_indexed];
+  split;
+  . intro h;
+    apply next_parametericConsistent (𝓢 := 𝓢);
+    assumption;
+  . tauto;
+
+lemma mem_lindenbaum_next_indexed (t) (φ : Formula α) : φ ∈ t[(encode φ) + 1].1 ∨ φ ∈ t[(encode φ) + 1].2 := by
+  simp [lindenbaum_next_indexed, lindenbaum_next];
+  split;
+  . left; tauto;
+  . right; tauto;
+
+lemma lindenbaum_next_indexed_parametricConsistent [System.Intuitionistic 𝓢] (consistent : t.Consistent 𝓢) (i : ℕ) : t[i].Consistent 𝓢 := by
+  induction i with
+  | zero => simpa;
+  | succ i ih => apply lindenbaum_next_indexed_parametricConsistent_succ; assumption;
+
+variable {m n : ℕ}
+
+lemma lindenbaum_next_indexed_subset₁_of_lt (h : m ≤ n) : t[m].1 ⊆ t[n].1 := by
+  induction h with
+  | refl => simp;
+  | step h ih =>
+    simp [lindenbaum_next_indexed, lindenbaum_next];
+    split;
+    . split <;> tauto;
+    . tauto;
+
+lemma lindenbaum_next_indexed_subset₂_of_lt (h : m ≤ n) : t[m].2 ⊆ t[n].2 := by
+  induction h with
+  | refl => simp;
+  | step h ih =>
+    simp [lindenbaum_next_indexed, lindenbaum_next];
+    split;
+    . split <;> tauto;
+    . tauto;
+
+lemma exists_parametricConsistent_saturated_tableau [System.Intuitionistic 𝓢] (hCon : t.Consistent 𝓢) : ∃ u, t ⊆ u ∧ (Tableau.Consistent 𝓢 u) ∧ (Saturated u) := by
+  use t∞;
+  refine ⟨?subset, ?consistent, ?saturated⟩;
+  case subset => constructor <;> apply Set.subset_iUnion_of_subset 0 (by simp);
+  case saturated =>
+    intro φ;
+    rcases mem_lindenbaum_next_indexed (𝓢 := 𝓢) t φ with (h | h);
+    . left; simp [lindenbaum_maximal]; use (encode φ + 1);
+    . right; simp [lindenbaum_maximal]; use (encode φ + 1);
+  case consistent =>
+    intro Γ Δ hΓ hΔ;
+    simp_all [lindenbaum_maximal];
+    obtain ⟨m, hΓ⟩ : ∃ m, ∀ φ ∈ Γ, φ ∈ t[m].1 := by
+      induction Γ with
+      | nil => simp;
+      | cons φ Γ ih =>
+        simp_all;
+        obtain ⟨i, hi⟩ := hΓ.1;
+        obtain ⟨m, hm⟩ := ih;
+        use (i + m);
+        constructor;
+        . exact lindenbaum_next_indexed_subset₁_of_lt (by simp) hi;
+        . intro ψ hq;
+          exact lindenbaum_next_indexed_subset₁_of_lt (by simp) $ hm ψ hq;
+    obtain ⟨n, hΔ⟩ : ∃ n, ∀ φ ∈ Δ, φ ∈ t[n].2 := by
+      induction Δ with
+      | nil => simp;
+      | cons φ Δ ih =>
+        simp_all;
+        obtain ⟨i, hi⟩ := hΔ.1;
+        obtain ⟨n, hn⟩ := ih;
+        use (i + n);
+        constructor;
+        . exact lindenbaum_next_indexed_subset₂_of_lt (by simp) hi;
+        . intro ψ hq;
+          exact lindenbaum_next_indexed_subset₂_of_lt (by simp) $ hn ψ hq;
+    rcases (lt_trichotomy m n) with hm | hmn | hn;
+    . exact lindenbaum_next_indexed_parametricConsistent hCon n (by intro φ hp; exact lindenbaum_next_indexed_subset₁_of_lt hm.le $ hΓ φ hp) hΔ;
+    . subst hmn;
+      exact lindenbaum_next_indexed_parametricConsistent hCon m hΓ hΔ;
+    . exact lindenbaum_next_indexed_parametricConsistent hCon m hΓ (by intro φ hp; exact lindenbaum_next_indexed_subset₂_of_lt hn.le $ hΔ φ hp);
+
+protected alias lindenbaum := exists_parametricConsistent_saturated_tableau
+
+end lindenbaum
+
+end Tableau
+
+
+open Tableau
+
+
+def SaturatedConsistentTableau (𝓢 : S) := {t : Tableau α // Saturated t ∧ t.Consistent 𝓢}
+
+namespace SaturatedConsistentTableau
+
+lemma consistent (t : SaturatedConsistentTableau 𝓢) : Consistent 𝓢 t.1 := t.2.2
+
+lemma saturated (t : SaturatedConsistentTableau 𝓢) : Saturated t.1 := t.2.1
+
+variable {t₀ : Tableau α} {φ ψ : Formula α}
+
+lemma lindenbaum [System.Intuitionistic 𝓢] [Encodable α] (hCon : t₀.Consistent 𝓢) : ∃ (t : SaturatedConsistentTableau 𝓢), t₀ ⊆ t.1 := by
+  obtain ⟨t, ht, hCon, hMax⟩ := Tableau.lindenbaum hCon;
+  exact ⟨⟨t, hMax, hCon⟩, ht⟩;
+
+instance [System.Consistent 𝓢] [System.Intuitionistic 𝓢] [DecidableEq α] [Encodable α] : Nonempty (SaturatedConsistentTableau 𝓢) := ⟨lindenbaum Tableau.emptyset_consistent |>.choose⟩
+
+variable {t t₁ t₂ : SaturatedConsistentTableau 𝓢}
+
+lemma not_mem₂ {Γ : List (Formula α)} (hΓ : ∀ φ ∈ Γ, φ ∈ t.1.1) (h : 𝓢 ⊢! ⋀Γ ➝ ψ) : ψ ∉ t.1.2 := t.1.not_mem₂ t.consistent hΓ h
+
+variable [System.Intuitionistic 𝓢]
+
+@[simp] lemma disjoint : Disjoint t.1.1 t.1.2 := t.1.disjoint_of_consistent t.2.2
+
+lemma not_mem₁_iff_mem₂ : φ ∉ t.1.1 ↔ φ ∈ t.1.2 := Tableau.not_mem₁_iff_mem₂ t.consistent t.saturated
+
+lemma not_mem₂_iff_mem₁ : φ ∉ t.1.2 ↔ φ ∈ t.1.1 := Tableau.not_mem₂_iff_mem₁ t.consistent t.saturated
+
+lemma saturated_duality: t₁.1.1 = t₂.1.1 ↔ t₁.1.2 = t₂.1.2 := Tableau.saturated_duality t₁.consistent t₂.consistent t₁.saturated t₂.saturated
+
+lemma equality_of₁ (e₁ : t₁.1.1 = t₂.1.1) : t₁ = t₂ := by
+  have e := Tableau.equality_def.mpr ⟨e₁, (saturated_duality.mp e₁)⟩;
+  calc
+    t₁ = ⟨t₁.1, t₁.saturated, t₁.consistent⟩ := by rfl;
+    _  = ⟨t₂.1, t₂.saturated, t₂.consistent⟩ := by simp [e];
+    _  = t₂                                  := by rfl;
+
+lemma equality_of₂ (e₂ : t₁.1.2 = t₂.1.2) : t₁ = t₂ := equality_of₁ $ saturated_duality.mpr e₂
+
+
+lemma mdp₁ (hp₁ : φ ∈ t.1.1) (h : 𝓢 ⊢! φ ➝ ψ) : ψ ∈ t.1.1 := by
+  apply not_mem₂_iff_mem₁.mp;
+  by_contra hq₂;
+  have : 𝓢 ⊬ φ ➝ ψ := by simpa using t.consistent (Γ := [φ]) (Δ := [ψ]) (by simpa) (by simpa);
+  contradiction;
+
+@[simp]
+lemma mem₁_verum : ⊤ ∈ t.1.1 := by
+  apply not_mem₂_iff_mem₁.mp;
+  by_contra hC;
+  have : 𝓢 ⊬ ⋀[] ➝ ⋁[⊤] := t.consistent (by simp) (by simpa);
+  have : 𝓢 ⊢! ⋀[] ➝ ⋁[⊤] := by simp;
+  contradiction;
+
+@[simp]
+lemma not_mem₁_falsum : ⊥ ∉ t.1.1 := by
+  by_contra hC;
+  have : 𝓢 ⊬ ⋀[⊥] ➝ ⋁[] := t.consistent (by simpa) (by simp);
+  have : 𝓢 ⊢! ⋀[⊥] ➝ ⋁[] := by simp;
+  contradiction;
+
+@[simp]
+lemma iff_mem₁_and : φ ⋏ ψ ∈ t.1.1 ↔ φ ∈ t.1.1 ∧ ψ ∈ t.1.1 := by
+  constructor;
+  . intro h; constructor <;> exact mdp₁ h (by simp)
+  . rintro ⟨hp, hq⟩;
+    apply not_mem₂_iff_mem₁.mp;
+    by_contra hC;
+    have : 𝓢 ⊢! ⋀[φ, ψ] ➝ ⋁[φ ⋏ ψ] := by simp;
+    have : 𝓢 ⊬ ⋀[φ, ψ] ➝ ⋁[φ ⋏ ψ] := t.consistent (by simp_all) (by simp_all);
+    contradiction;
+
+lemma iff_mem₁_conj {Γ : List (Formula α)} : ⋀Γ ∈ t.1.1 ↔ ∀ φ ∈ Γ, φ ∈ t.1.1 := by
+  induction Γ using List.induction_with_singleton with
+  | hnil => simp [-top_def];
+  | hsingle φ => simp;
+  | hcons φ Γ Γ_nil ih =>
+    simp only [(List.conj₂_cons_nonempty Γ_nil), List.mem_cons];
+    constructor;
+    . rintro h φ (rfl | hp);
+      . exact iff_mem₁_and.mp h |>.1;
+      . exact ih.mp (iff_mem₁_and.mp h |>.2) _ hp;
+    . intro h;
+      apply iff_mem₁_and.mpr;
+      simp_all;
+
+@[simp]
+lemma iff_mem₁_or : φ ⋎ ψ ∈ t.1.1 ↔ φ ∈ t.1.1 ∨ ψ ∈ t.1.1 := by
+  constructor;
+  . intro h;
+    by_contra hC; push_neg at hC;
+    have : φ ∈ t.1.2 := not_mem₁_iff_mem₂.mp hC.1;
+    have : ψ ∈ t.1.2 := not_mem₁_iff_mem₂.mp hC.2;
+    have : 𝓢 ⊢! ⋀[φ ⋎ ψ] ➝ ⋁[φ, ψ] := by simp;
+    have : 𝓢 ⊬ ⋀[φ ⋎ ψ] ➝ ⋁[φ, ψ] := t.consistent (by simp_all) (by simp_all);
+    contradiction;
+  . intro h;
+    cases h with
+    | inl h => exact mdp₁ h or₁!
+    | inr h => exact mdp₁ h or₂!
+
+lemma not_mem₁_neg_of_mem₁ [DecidableEq α] : φ ∈ t.1.1 → ∼φ ∉ t.1.1 := by
+  intro hp;
+  by_contra hnp;
+  have := iff_mem₁_and.mpr ⟨hp, hnp⟩;
+  have : ⊥ ∈ t.1.1 := mdp₁ this intro_bot_of_and!;
+  have : ⊥ ∉ t.1.1 := not_mem₁_falsum
+  contradiction;
+
+lemma mem₂_neg_of_mem₁ [DecidableEq α] : φ ∈ t.1.1 → ∼φ ∈ t.1.2 := by
+  intro h;
+  exact not_mem₁_iff_mem₂ (φ := ∼φ) (t := t) |>.mp $ not_mem₁_neg_of_mem₁ h;
+
+lemma mem₁_of_provable : 𝓢 ⊢! φ → φ ∈ t.1.1 := by
+  intro h;
+  exact mdp₁ mem₁_verum $ imply₁'! h;
+
+lemma mdp₁_mem [DecidableEq α] (hp : φ ∈ t.1.1) (h : φ ➝ ψ ∈ t.1.1) : ψ ∈ t.1.1 := by
+  apply not_mem₂_iff_mem₁.mp;
+  by_contra hC;
+  have : 𝓢 ⊬ (φ ⋏ (φ ➝ ψ)) ➝ ψ := t.consistent (Γ := [φ, φ ➝ ψ]) (Δ := [ψ]) (by aesop) (by simpa);
+  have : 𝓢 ⊢! (φ ⋏ (φ ➝ ψ)) ➝ ψ := mdp_in!
+  contradiction;
+
+end SaturatedConsistentTableau
