Foundation/IntProp/Kripke2/Hilbert/Int.lean
@@ -1,4 +1,5 @@
 import Foundation.IntProp.Hilbert2.Int
+import Foundation.IntProp.Kripke2.Completeness
 import Foundation.IntProp.Kripke2.Hilbert.Soundness
 
 namespace LO.IntProp
@@ -12,6 +13,10 @@ namespace Hilbert.Int.Kripke
 instance sound : Sound Hilbert.Int AllFrameClass := inferInstance
 
 instance consistent : System.Consistent Hilbert.Int := Kripke.Hilbert.consistent_of_FrameClass AllFrameClass
+
+instance canonical : Canonical Hilbert.Int AllFrameClass := by tauto;
+
+instance complete: Complete Hilbert.Int AllFrameClass := inferInstance
 
 end Hilbert.Int.Kripke
 
