Foundation/IntProp/Kripke2/Hilbert/LC.lean
@@ -1,8 +1,10 @@
 import Foundation.IntProp.Hilbert2.WellKnown
 import Foundation.IntProp.Kripke2.Hilbert.Soundness
+import Foundation.IntProp.Kripke2.Completeness
 
 namespace LO.IntProp
 
+open Kripke
 open Formula.Kripke
 
 abbrev Kripke.ConnectedFrameClass : FrameClass := { F | Connected F }
@@ -31,11 +33,10 @@ instance : Kripke.ConnectedFrameClass.DefinedByFormula (Axioms.Dummett (.atom 0)
 
 
 instance : Kripke.ConnectedFrameClass.IsNonempty := ⟨by
-  use ⟨Unit, λ _ _ => True, by simp [Reflexive], by simp [Transitive]⟩;
+  use pointFrame;
   simp [Connected];
 ⟩
 
-open Kripke
 
 namespace Hilbert.LC.Kripke
 
@@ -44,6 +45,31 @@ instance : ConnectedFrameClass.DefinedBy (Hilbert.LC.axioms) := FrameClass.defin
 instance sound : Sound Hilbert.LC ConnectedFrameClass := inferInstance
 
 instance consistent : System.Consistent Hilbert.LC := Kripke.Hilbert.consistent_of_FrameClass ConnectedFrameClass
+
+open
+  System
+  SaturatedConsistentTableau
+in
+instance canonical : Canonical Hilbert.LC ConnectedFrameClass := by
+  constructor;
+  simp [Connected, Kripke.canonicalFrame];
+  intro x y z Rxy Ryz;
+  apply or_iff_not_imp_left.mpr;
+  intro nRyz;
+  obtain ⟨φ, hyp, nhzp⟩ := Set.not_subset.mp nRyz;
+  intro ψ hqz;
+  have : ψ ➝ φ ∉ x.1.1 := by
+    by_contra hqpx;
+    have hqpz : ψ ➝ φ ∈ z.1.1 := by aesop;
+    have : φ ∈ z.1.1 := mdp₁_mem hqz hqpz;
+    contradiction;
+  have := iff_mem₁_or.mp $ mem₁_of_provable (t := x) (φ := (φ ➝ ψ) ⋎ (ψ ➝ φ)) dummett!;
+  have hpqx : φ ➝ ψ ∈ x.1.1 := by aesop;
+  have hpqy : φ ➝ ψ ∈ y.1.1 := Rxy hpqx;
+  have : ψ ∈ y.1.1 := mdp₁_mem hyp hpqy;
+  exact this;
+
+instance complete : Complete Hilbert.LC ConnectedFrameClass := inferInstance
 
 end Hilbert.LC.Kripke
 
